\documentclass[12pt,a4paper]{scrreprt}
\usepackage{tikz}
\usetikzlibrary{positioning,calc}
\usepackage{amsmath,amssymb,mathrsfs,dsfont}
\usepackage[utf8]{inputenc}
\usepackage[ngerman]{babel}
\usepackage[colorlinks=false, pdfborderstyle={/S/U/W 1}
]{hyperref}
\usepackage{stmaryrd}
\usepackage{comment}
\oddsidemargin0mm \evensidemargin3mm \textwidth150mm \textheight23cm
\parindent0mm \pagestyle{empty} \topmargin-1cm
\newcommand{\E}{\mathds{E}}
\newcommand{\V}{\mathds{V}}
\newcommand{\C}{\mathds{C}}
\newcommand{\N}{\mathds{N}}
\newcommand{\Z}{\mathds{Z}}
\newcommand{\R}{\mathds{R}}
\pagestyle{headings}


\newcommand{\Lsg}{\textbf{Lsg.:}}

\begin{document}

\begin{flushleft}
\href{mailto:anja.voss-boehme@htw-dresden.de}{Prof. Dr. Anja Voß-Böhme} \\
\href{mailto:buder@htw-dresden.de}{Dipl.-Math. Thomas Buder}
\end{flushleft}

\begin{center}{\large\textbf Wirtschaftsmathematik II} \\ SS 2015 \end{center}

\begin{center}{\large\textbf{Übung 12}} 
\end{center}

\begin{tabular}{ll}
$a$		&	$ax$ 	\\
$x^n$	&	$\frac{1}{n+y}x^{x+1}$	\\
$e^x$	&	$e^x$	\\
$\frac{1}{x}$	&	$\ln|x|$	\\
$\sin x$	&	$-\cos x$	\\
$\cos x$	&	$\sin x$	\\
\end{tabular}


\[
\int{f \cdot f(x)} dx	=	\int f(x) dx \\
\int f(x)+g(x) dx	=	\int f(x) dx + \int g(x) dx	\\
\]

\begin{enumerate}

\item	%1.

\begin{enumerate}

\item %a

\[
\int 4x^3 +3x^2 +1	dx\\
=	4\frac{1}{4}x^4 +4\frac{1}{3}x^3 +x +c \\
= x^4 + x^3 +x +c
\]

\item %b

\[
\int \cos x + \sin(2x) +\frac{1}{x} -\frac{e^x}{2}	dx\\
= \sin x + \int \sin(2x) dx + \ln |x| -\frac{1}{2}e^x \\
z = \int \sin(2x) dx \\
dz = 2dx \\
dx=\frac{dz}{2} \\
\int z dx = \int \sin z \frac{dz}{2} = \frac{1}{2} \int \sin z dz = -\frac{1}{2}\cos z \rightarrow -\frac{1}{2}\cos 2x \\
\]

\item %c

\[
\int (3x+4)^3 dx \\
z=3x+4 \\
1 dz = 3dx \\
dx = \frac{dz}{3} \\
\frac{1}{3} \int z^3 dz = \frac{1}{3} \frac{1}{4} z^4 = \frac{1}{12} (3x+4)^4
\]

\item %d

\[
\int \frac{e^x}{1-e^x} \\
z = 1-e^x \\
dz = -e^x dx
dx = \frac{dz}{-e^x}
\int \frac{e^x}{z} \\
= \int \frac{e^x}{z} \frac{dz}{e^x} = \int \frac{1}{z} dz \\
= -\ln|z| = -\ln |1-e^x|
\]

\item %e

\[
\int x(x^2+10)^2 5  dx \\
= 5(\frac{1}{6}x^6 +5x^4 +50x^2)
\]

\item %f

\[
\int x \ln x dx
= \int u'v = uv-\int uv' dx
u'=x
v =\ln x
u =\frac{1}{2}x^2
v'=\frac{1}{x}
\frac{1}{2}x^2 \ln x -\frac{1}{2}\int x^2 \frac{1}{x} dx
= \frac{1}{2}x^2 \ln x -\frac{1}{2}\frac{1}{2}x^2
= \frac{1}{2}x^2 \ln x -\frac{1}{4}x^2
\]

\item %g

\[
\int x+\ln x dx
= \int u'v = uv-\int uv'
u'=1
v =\ln x
u =x
v'=\frac{1}{x}
x \cdot \ln x -\int x \frac{1}{x} dx
= x \ln x -\int 1 dx
= x \ln x -x
=x(\ln x -1)
\]

\item %h

\[
\int x^2 e^{3x} dx
= \int u'v = uv-\int uv'
u'=e^{3x}
v =x^2
u =\frac{1}{3} e^{3x}
v'=2x
= \int e^{3x} x^2 = \frac{1}{3} e^{3x} x^2 -\frac{2}{3} \int e^{3x} x dx
u'=e^{3x}
v =x
u =\frac{1}{3}e^{3x}
v'=1
\int e^{3x} x dx = \frac{1}{3}e^{3x}-\frac{1}{3}\frac{1}{3}e^{3x}
\int x^2 e^{3x} dx = \frac{1}{3} e^{3x} x^2 -\frac{2}{9}e^{3x}-\frac{1}{9}e^{3x}
\]

\end{enumerate}

\item %2

\[
K'(x)=6x^2 -2x +20 \\K
K(10)=6000
K(x)=\int K'(x) dx
= 2x^3 -1x^2 +20x +c
K(10)=2100 +c=6000
c=6000-2100=3900
K(x)=2x^3 -1x^2 +20x +3900
\]

\item %3

\[
K'(x)=e^x+x^2
K(x)=\int K'(x) dx
Fixosten = 1200 \Rightarrow c: K(0)=1200
K(x)=e^x + \frac{1}{3}x^3+c
K(0)=1 + c=1200
c=1199
K(x)=e^x + \frac{1}{3}x^3 +1199
\]

\item %4

\[
A=\int_a^b f(x) dx
\]

\[
f(x)=2\ln \left(x+\frac{1}{2}\right)
0=2\ln \left(x+\frac{1}{2}\right)	|\cdot e^z
x=\frac{1}{2}
\]

\[
\left| \int_{0}^{x_{0}} 2\ln \left(x+\frac{1}{2}\right) dx \right| \\
= \left| 2 \int_{\frac{1}{2}}^{1} \ln z ~dz \right|
= | 2 [ z (\ln z-1 ) ] |
= | 2 (1(\ln 1-1)) - 2(\frac{1}{2}(\ln \frac{1}{2}-1)) |
= |-2 - \ln \frac{1}{2} +1 |
= |-1 -\ln \frac{1}{2} |
= 1+\ln\frac{1}{2}
= 1+\ln 2^{-1}
= 1-\ln 2
\]

\item %5

\[
f_k(x)=\frac{1}{k}(2x^3-x)
\]

\[
f_k(x)=0
\]

\[
0=2x^3-x
=x(2x^2-1) \rightarrow x_0=0
\]

\[
0=2x^2-1
\]

\[
x_{1,2}=\pm \sqrt{\frac{1}{2}} 
\]

\[
A=\left|\int_{0}^{\sqrt{\frac{1}{2}}} \frac{1}{k}(2x^3-x) dx\right|
= \left| \frac{1}{k} \left[ \frac{1}{2}x^4-\frac{1}{2}x^2 \right]_{0}^{\sqrt{\frac{1}{2}}} \right|
\]

\[
= \left| \frac{1}{k} \left(\frac{1}{2}\frac{1}{4}-\frac{1}{4}\right)-\frac{1}{k}(0) \right|
= \left| \frac{1}{k} \left(\frac{1}{8}-\frac{1}{4}\right) \right|
= \left|- \frac{1}{k} \frac{1}{9} \right|
= \frac{1}{8k}
\]

\end{enumerate}

\end{document}
